Get some examples working (TODO: clean up file)

src/Utils/RelationalDB.v
@@ -24,23 +24,45 @@ Open Scope positive.
   (*TODO: use something other than list? for our uses list might be optimal,
     depending on how it's generated
    *)
-  Inductive query_trie :=
-  (*TODO!!!: what is the difference between qt_nil and qt_tree []
-  | qt_nil*)
+Inductive query_trie :=
+  (*Necessary for when a variable does not appear in a clause *)
+  | qt_unconstrained : query_trie -> query_trie
   (* need to expose map impl or inductive is not strictly positive *)
   | qt_tree : TrieMap.map query_trie -> query_trie.
 
   Notation qt_nil := (qt_tree (PTree.Empty)).
-  
-  Definition values_of_next_var (t : query_trie) :  list positive :=
-    let (m) := t in
-    map.fold (fun l k _ => cons k l) [] m.
+
+
+Instance trie_set : set positive :=
+  {
+    set_as_map := TrieMap.map _;
+    intersection := PTree.combine (fun a b => if a then b else None);
+    union := PTree.combine (fun a b => if a then Some tt else b);
+  }.
+
+(* Includes top element, isomorphic to option *)
+Variant pos_set := finite_set (m : trie_set) | all_positives.
+
+Definition pos_set_intersection p1 p2 :=
+  match p1, p2 with
+  | finite_set s1, finite_set s2 => finite_set (intersection s1 s2)
+  | finite_set s1, all_positives => finite_set s1
+  | all_positives, finite_set s2 => finite_set s2
+  | all_positives, all_positives => all_positives
+  end.
+
+Definition values_of_next_var (t : query_trie) : pos_set :=
+  match t with
+  | qt_tree m => finite_set (PTree.map_filter (fun _ => Some tt) m)
+  | qt_unconstrained _ => all_positives
+  end.
   
   Definition choose_next_val (v:positive) (t : query_trie) : query_trie :=
-    let (m) := t in
-    match map.get m v with Some t => t | None => qt_nil end.
-    
-
+  match t with
+  | qt_tree m => 
+    match map.get m v with Some t => t | None => qt_nil end
+  | qt_unconstrained t => t 
+  end.   
 
   Fixpoint list_compare l1 l2 :=
     match l1, l2 with
@@ -99,18 +121,35 @@ Open Scope positive.
   (* TODO: figure out whether this can have duplicates
      {subst_set : set arg_map}.
    *)
-  Definition subst_set := list arg_map.
+Definition subst_set := list arg_map.
 
-  Fixpoint generic_join' (tries : @named_list Idx query_trie)
-           (vars : list Idx) (acc : arg_map) : subst_set :=
-    match vars with
-    | [] => [acc]
-    | (x::vars') =>
-        let Dx := flat_map (fun '(_,v) => values_of_next_var v) tries in
-        flat_map (fun v => generic_join' (named_map (choose_next_val v) tries) vars'
-                                         (map.put acc x v))
-                 Dx
-    end.
+(*TODO: move to extramaps/Triemap *)
+Definition as_list {A} :=
+  TrieMap.trie_fold (B:=A) (fun m k v => (k,v)::m) [].
+
+  
+
+Fixpoint generic_join' (tries : @named_list Idx query_trie)
+         (vars : list Idx) (acc : arg_map) : subst_set :=
+  match vars with
+  | [] => [acc]
+  | (x::vars') =>
+      let Rxs : list pos_set :=
+        map (fun '(_,v) => values_of_next_var v) tries in
+      let Dx := fold_left pos_set_intersection Rxs all_positives in
+      (*
+        If Dx is all_positives, then the variable is unconstrained.
+        We will probably only guarentee the behavior of generic_join
+        when all free variables appear, so the result in this case doesn't matter
+       *)
+      match Dx with
+      | finite_set Dx =>
+          flat_map (fun v => generic_join' (named_map (choose_next_val v) tries) vars'
+                                           (map.put acc x v))
+                   (map fst (as_list Dx))
+      | all_positives => []
+      end
+  end.
   
 
   (* we need constants for residual queries in generic_join *)
@@ -145,12 +184,31 @@ Definition match_args_and_lookup args tuple (x : Idx) : option elt :=
      let e <- map.get m x in
      ret e.
 
-  Definition find_values_in_relation (x : Idx) (rel : relation) args :=
+  Definition find_values_in_relation' (x : Idx) (rel : relation) args :=
     map.fold (fun acc tuple _ =>
                 match match_args_and_lookup args tuple x with
                 | Some e => e::acc
                 | None => acc
                 end) [] rel.
+
+#[refine]
+Instance eqb_argument : Eqb argument :=
+  {
+    eqb a b :=
+    match a,b with
+    | var_arg ax, var_arg bx => eqb ax bx
+    | const_arg ac, const_arg bc => eqb ac bc
+    | _,_ => false
+    end;
+  }.
+all: eapply TODO.
+Defined.
+
+(*handle unconstrained variables*)
+Definition find_values_in_relation (x : Idx) (rel : relation) args :=
+  if existsb (eqb (var_arg x)) args
+  then Some (find_values_in_relation' x rel args)
+  else None.
 
   Definition arg_subst v x a :=
     match a with
@@ -163,18 +221,24 @@ Goal (arg_subst 2 1 (var_arg 1) = const_arg 2). reflexivity. Qed.
 Goal (arg_subst 2 1 (var_arg 3) = var_arg 3). reflexivity. Qed.
 Goal (arg_subst 2 1 (const_arg 1) = const_arg 1). reflexivity. Qed.
   
-  (*TODO: filter rel on recursive calls?*)
+(*TODO: filter rel on recursive calls?*)
+(* TODO: if a variable is unconstrained, need to handle it specially *)
 Fixpoint build_trie' (rel: relation) (vars : list Idx) (args : list argument)
   : query_trie :=
     match vars with
     | [] => qt_nil
     | x::vars' =>
         let vs := find_values_in_relation x rel args in
-        qt_tree (fold_left
-                   (fun m v =>
-                      map.put m v (build_trie' rel vars' (map (arg_subst v x) args)))
-                   vs
-                   map.empty)
+        match vs with
+        | Some vs =>
+            qt_tree (fold_left
+                       (fun m v =>
+                          map.put m v (build_trie' rel vars' (map (arg_subst v x) args)))
+                       vs
+                       map.empty)
+        | None  =>
+            qt_unconstrained (build_trie' rel vars' args)
+        end
     end.
 
   Definition build_trie (d:db) (vars : list Idx) (clause : atom) : Idx * query_trie :=
@@ -203,15 +267,15 @@ Definition build_tries (d:db) (vars : list Idx) (clauses : list atom)
         [6; 4; 5].
 
 
-    Goal find_values_in_relation 1 r1 [var_arg 1; var_arg 2; var_arg 1] = [].
+    Goal find_values_in_relation 1 r1 [var_arg 1; var_arg 2; var_arg 1] = Some [].
       Proof. reflexivity. Qed.
-    Goal find_values_in_relation 1 r1 [var_arg 1; var_arg 2; var_arg 3] = [6; 10].
+    Goal find_values_in_relation 1 r1 [var_arg 1; var_arg 2; var_arg 3] = Some [6; 10].
       Proof. reflexivity. Qed.
-    Goal find_values_in_relation 1 r1 [var_arg 2; var_arg 1; var_arg 1] = [20].
+    Goal find_values_in_relation 1 r1 [var_arg 2; var_arg 1; var_arg 1] = Some [20].
       Proof. reflexivity. Qed.
-    Goal find_values_in_relation 1 r1 [var_arg 1; var_arg 1; var_arg 2] = [].
+    Goal find_values_in_relation 1 r1 [var_arg 1; var_arg 1; var_arg 2] = Some [].
       Proof. reflexivity. Qed.
-    Goal find_values_in_relation 1 r1 [var_arg 1; var_arg 1; var_arg 1] = [].
+    Goal find_values_in_relation 1 r1 [var_arg 1; var_arg 1; var_arg 1] = Some [].
       Proof. reflexivity. Qed.
     
     Definition r2 : relation :=
@@ -245,16 +309,54 @@ Definition build_tries (d:db) (vars : list Idx) (clauses : list atom)
                   [(1,[1;2;3]);(3,[2;2;3])].
  
     
-    Definition as_list {A} :=
-      TrieMap.trie_fold (B:=A) (fun m k v => (k,v)::m) [].
 
     Definition tries := Eval compute in  (build_tries db_ex q1.(free_vars) q1.(clauses)).
 
-    Compute (map as_list (generic_join' tries q1.(free_vars) map.empty)).
+    Compute (map as_list (generic_join' tries q1.(free_vars) map.empty)). 
     
-    (*TODO: duplicates some results; should actually use a set?
-      Variable ordering seems to affect this
-     *)
-    (*TODO: bug when a var isn't mentioned in all clauses*)
     Compute (map as_list (generic_join db_ex q1)).
 
+    (*TODO: for debugging only*)
+    Definition pos_set_as_list (p:pos_set) :=
+      match p with
+      | all_positives => None (*TODO: change if causes debugging confusion*)
+      | finite_set m => Some (map fst (as_list m))
+      end.
+
+    (*TODO: 3 should be unconstrained*)
+    (* tries seem to be generated correctly *)
+    Compute (named_map (fun t =>
+                          (pos_set_as_list (values_of_next_var t
+                       )))
+                       tries). 
+
+    Compute (intersection (set:=trie_set) (map.singleton 2 tt) (map.singleton 2 tt)).
+
+    Let vars := Eval compute in q1.(free_vars).
+    Let acc:arg_map := map.empty.
+
+    Let Rxs := Eval compute in (map (fun '(_,v) => values_of_next_var v) tries).
+    Compute (map as_list Rxs).
+    Let Dx := Eval compute in ( fold_left intersection Rxs map.empty).
+
+  Fixpoint generic_join' (tries : @named_list Idx query_trie)
+           (vars : list Idx) (acc : arg_map) : subst_set :=
+    match vars with
+    | [] => [acc]
+    | (x::vars') =>
+        let Rxs : list trie_set :=
+          map (fun '(_,v) => values_of_next_var v) tries in
+        (*If Rxs is empty then there are no tries, i.e. no clauses
+          In theory, this should allow the variables to range over all values
+          This is impractical with an infinite set.
+          TODO: determine what to do in this case based on what makes the proof easy
+         *)
+        match Rxs with
+        | [] => []
+        | Rx1::Rxs =>
+            let Dx := fold_left intersection Rxs Rx1 in
+            flat_map (fun v => generic_join' (named_map (choose_next_val v) tries) vars'
+                                             (map.put acc x v))
+                     (map fst (as_list Dx))
+        end
+    end.
